`eUnion_MFacts`

coq/SigmaHCOL/MSigmaHCOL.v
@@ -1435,8 +1435,9 @@ Section MSHOperator_Definitions.
                       (Full_set _).
 
   Definition MSHeUnion
-             {svalue: CarrierA}
+             (svalue: CarrierA)
              {o b: nat}
+             (bc: b < o)
     := @mkMSHOperator 1 o
                       (eUnion_mem b)
                       eUnion_mem_proper
@@ -1736,7 +1737,71 @@ Section MSHOperator_Facts_instances.
       break_match_hyp; try some_none.
       pose proof (out_mem_oob  m1 H) as P2.
       apply P2; auto.
-  Defined.
+  Qed.
+
+  Global Instance eUnion_MFacts
+         {svalue: CarrierA}
+         {o b: nat}
+         (bc: b < o)
+  : MSHOperator_Facts (MSHeUnion svalie bc).
+  Proof.
+    unshelve esplit.
+    -
+      (* mem_out_some *)
+      intros m H.
+      unfold is_Some, MSHeUnion, eUnion_mem, map_mem_block_elt, mem_lookup. simpl.
+      repeat break_match; try some_none; try tauto.
+      clear Heqo0. rename Heqo1 into M.
+      simpl in *.
+      assert(P: Full_set (FinNat 1) (mkFinNat Nat.lt_0_1)) by apply Full_intro.
+      apply H in P.
+      unfold mem_lookup, mem_in in *.
+      apply NP.F.not_find_in_iff in M.
+      congruence.
+    -
+      (* out_mem_fill_pattern *)
+      intros m0 m H.
+      split.
+      +
+        simpl in *.
+        unfold eUnion_mem, map_mem_block_elt, mem_lookup, mem_in, mem_add, mem_empty in *.
+        break_match_hyp; try some_none.
+        some_inv.
+        subst m.
+        intros O.
+        destruct (eq_nat_dec j b).
+        --
+          apply NP.F.in_find_iff.
+          rewrite NP.F.add_eq_o; auto.
+          some_none.
+        --
+          unfold FinNatSet.singleton, mkFinNat in O.
+          simpl in O.
+          congruence.
+      +
+        simpl in *.
+        unfold eUnion_mem, map_mem_block_elt, mem_lookup, mem_in, mem_add, mem_empty in *.
+        break_match_hyp; try some_none.
+        some_inv.
+        subst m.
+        intros I.
+        unfold FinNatSet.singleton, mkFinNat.
+        destruct (eq_nat_dec j b); auto.
+        exfalso.
+        apply NP.F.in_find_iff in I.
+        rewrite NP.F.add_neq_o in I ; auto.
+    -
+      intros m0 m H j jc C.
+      simpl in H.
+      unfold eUnion_mem, map_mem_block_elt, mem_lookup, mem_in in *. simpl in *.
+      break_match; try some_none.
+      some_inv.
+      subst m.
+      unfold mem_add, mem_empty in C.
+      destruct (eq_nat_dec j b); try omega.
+      apply NP.F.in_find_iff in C.
+      rewrite NP.F.add_neq_o in C; auto.
+  Qed.
 
 
 End MSHOperator_Facts_instances.
